src/coq/Semantics/InfiniteToFinite.v
@@ -13220,6 +13220,7 @@ intros addr_fin addr_inf ms_fin ms_inf byte_inf byte_fin MSR ADDR_CONV BYTE_REF 
     generalize dependent ms_fin_start.
     generalize dependent ms_fin_final.
     induction TYPE_INF; intros ms_fin_final ms_fin_start ms_inf_start MSR bytes_fin uv_fin UV_REF SERIALIZE TYPE_FIN.
+
     all: try solve
         [ rewrite Memory64BitIntptr.MMEP.MemSpec.MemHelpers.serialize_sbytes_equation in SERIALIZE;
           rewrite MemoryBigIntptr.MMEP.MemSpec.MemHelpers.serialize_sbytes_equation;
